---
pagetitle: "Derivatives of Inverse Functions - Exploring Calculus"
---
# "Derivatives of Inverse Functions"

## Inverse Functions

In this section we state the derivative rules for the natural exponential function and the general exponential function. 
We also go over several examples of the chain rule and the exponential derivative rules.


::: {#thm- } 
\index{derivative of inverse} **derivative of inverse** 
If $f$ has an interval $I$ as domain and $f'(x)$ exists and is never zero on $I,$ then $f^{-1}$ is differentiable at every point in its domain. 
The value of $\left(f^{-1}\right)'$ at a point $b$ in the domain of $f^{-1}$ is the reciprocal of the value of $f'$ at $a=f^{-1}(b)$ given by  
\[
\left(f^{-1}\right)'(b)=\frac{1}{f '\left(f^{-1}(b)\right)}.
\]
::: 


::: {#exm- } 
Let $\ds f(x)=\frac{2x-3}{7-5x}.$ 
Sketch the graph of $f$ and state whether or not the graph of $f$ passes the horizontal line test. 
If so, find a rule for $f^{-1}$ and then use it to find $\left(f^{-1}\right) '(0)$. 
Verify the formula
\[
\ds \left(f^{-1}\right)'(0)=\frac{1}{f'\left(f^{-1}(0)\right)}.
\]
::: 

\begin{figure}[htbp]
\begin{center}
{\includegraphics[width=250pt]{_includes/p20.pdf}} 
\caption{The graph of $\ds f(x)=\frac{2x-3}{7-5x}.$.}
\label{fig:}
\end{center}
\end{figure}

::: {.solution }
Notice that the graph of $f$ passes the horizontal line test, which implies that $f$ is a one-to-one function and thus must have an inverse function. 
To find the inverse function of $f$, set $y=f(x)$. 
Then simply switch the variables $x$ and $y$ and solve for $y$. 
The resulting equation will be a rule for the function $f^{-1}$. 
To see this, let $y=\frac{2x-3}{7-5x}$ and then switching the variables $x$ and $y$: $x=\frac{2y-3}{7-5y}$. 
Solving for $y$ yields: $y=\frac{3+7x}{2+5x}$. 
Thus, $f^{-1}(x)=\frac{3+7x}{2+5x}$. 
Of course since $f$ and $f^{-1}(x)$ are inverse function it must happen that $f^{-1}(f(x))=x$ and  $f(f^{-1}(x))=x$ for each $x$ in the domains. 
Notice that 
\[
f'(x)=-\frac{1}{(7-5 x)^2}  \qquad \text{and} \qquad (f^{-1})'(x)=-\frac{1}{(2+5 x)^2}.
\]
Also notice that 
\[
(f^{-1})'(0)=-\frac{1}{(2+5 (0))^2}=-\frac{1}{4}=\frac{1}{f'\left(\frac{3}{2}\right)}=\frac{1}{f'\left(f^{-1}(0)\right)}.
\]
::: 


::: {#exm- } 
Let $\ds f(x)=\frac{5 x}{1-2x}.$ 
Without finding a rule for $f^{-1}(x)$ determine $\left(f^{-1}\right) '(1).$
::: 

::: {.solution }
Since $\ds f'(x)=\frac{5}{(1-2 x)^2}$ and $\ds 1=\frac{5 x}{1-2x}$ when $x=\frac{1}{7}$
\[
\left(f^{-1}\right)'(1)=\frac{1}{f '\left(f^{-1}(1)\right)}=\frac{1}{f '(1/7)}=\frac{1}{\frac{49}{5}}=\frac{5}{49}.
\square
\]
::: 

## Derivatives of Exponential Functions


::: {#thm- } 
The derivative of the \index{exponential function} **exponential function**  $f(x)=b^x$ is $  f'(x)=(\ln  b) b^x.$ 
In the special case when $b=e$ we have $f(x)=e^x$ and $f'(x)=e^x.$ 
Therefore, 
\[
\frac{d}{dx}\left(b^x\right)=(\ln  b)b^x \qquad \text{and} \qquad \frac{d}{dx}\left(e^x\right)=e^x.
\]
::: 

::: {#exm- } 
Find the derivative of the function given $y(x)=x^2-3e^x.$
::: 

::: {.solution }
The derivative is $  \frac{dy}{dx}=2x-3e^x.$
::: 


::: {#exm- }  
Find the derivative of the function given $y(x)=1-2e^{-x^2}.$
::: 

::: {.solution }
Using the chain rule the derivative is,  
\[
\frac{dy}{dx}=-2e^{-x^2}\frac{d}{dx}\left(-x^2\right)=-2e^{-x^2}(-2x)=4x e^{-x^2}.
\square
\]
::: 

::: {#exm- } 
What is the slope of the tangent line to $\ds y=\frac{e^{-x}}{1+e^{-x}}$ at $x=0?$
::: 

::: {.solution }
Using the quotient rule,
\begin{align*}
\frac{dy}{dx}& =\frac{\left(1+e^{-x}\right)\left(-e^{-x}\right)-e^{-x}\left(-e^{-x}\right)}{\left(1+e^{-x}\right)^2} \\
& =\frac{-e^{-x}\left(1+e^{-x}-e^{-x}\right)}{\left(1+e^{-x}\right)^2} 
 =\frac{-e^{-x}}{\left(1+e^{-x}\right)^2}=-\frac{e^x}{\left(1+e^x\right)^2}
\end{align*}
Therefore, the slope of the tangent line to $y$ at $x=0$ is $  \frac{-e^{-(0)}}{\left(1+e^{-(0)}\right)^2}=-\frac{1}{4}.$
::: 


## Derivatives of Logarithmic Functions


::: {#thm- } 
The derivative of the \index{logarithmic function} **logarithmic function**  $f(x)=\log _bx$ is $  f'(x)=1/(\ln  b) x.$ 
In the special case when $b=e$ we have $f(x)=\ln  x$ and $f'(x)=1/x.$ 
Therefore, 
\[
\frac{d}{dx}\left(\log _bx\right)=\frac{1}{(\ln  b)x} \qquad \text{and} \qquad \frac{d}{dx}(\ln  x)=\frac{1}{x}.
\]
::: 


::: {#exm- } 
Find the equation of the tangent line to the curve $y=x^{2 }\ln  x $ at $x=e^2.$
::: 

::: {.solution }
The derivative of $y$ is $y'=2x \ln  x+x$ and at $\left(e^2,2 e^4\right)$ we have the slope of the tangent line as $y'\left(e^2\right)=2\left(e^2\right) \ln  \left(e^2\right)+\left(e^2\right)=5 e^2.$ 
Therefore, the equation of the tangent line is $y-2e^4=5e^2\left(x-e^2\right)$ which simplifies to $y=5 e^2 x-3 e^4.$
::: 


::: {#exm- } 
For what values of $A$ and $B$ does $y=A x \ln  x+B e^x$ satisfy $y''-y=0?$
::: 

::: {.solution }
We determine, $y'=A \ln  x+A+B e^x$ $y\text{''}=\frac{A}{x}+B e^x$. 
Since $y''-y=\frac{A}{x}-A x \ln  x=0$ we find that $A=0$ and that $B$ can be any real number.
::: 


::: {#exm- } 
Find the derivative of the function given by $y(x)=5^{2x^2}\ln (4x).$
::: 

::: {.solution }
Using the product rule and the chain rule,  
\begin{align*}
\frac{dy}{dx} & =\frac{d}{dx}\left(5^{2x^2}\right)\ln (4x)+5^{2x^2}\frac{d}{dx}(\ln (4x)) \\
& =\left(5^{2x^2}\ln (5)(4x)\right) \ln (4x)+5^{2x^2}\left(\frac{1}{4x}(4)\right)
\square 
\end{align*}
::: 

::: {#exm- } 
Find the derivative of the function given by $y(x)=\ln (4x+9).$
::: 

::: {.solution }
Using the chain rule,  
\[
\frac{dy}{dx}=\frac{1}{4x+9}\frac{d}{dx}(4x+9)=\frac{4}{4x+9}.
\square
\]
::: 

::: {#exm- } 
Find the derivative of the function given by 
\[
y(x)=\ln \left(\frac{x^3}{x+1}\right).
\]
::: 

::: {.solution }
Here we simplify first to have,  
\[
y(x)=\ln \left(\frac{x^3}{x+1}\right)=\ln \left(x^3\right)-\ln (x+1)=3 \ln (x)-\ln (x+1)
\]
and then using derivative rules,  
\[
\frac{dy}{dx}=\frac{3}{x}-\frac{1}{x+1}=\frac{2 x+3}{x (x+1)}.
\square
\]
::: 

::: {#exm- } 
Find the derivative of the function given by 
\[
y(x)=\log _2\left(\frac{3x+2}{x^2-5}\right){}^{1/4}.
\]
::: 

::: {.solution }
Here we simplify first to have,  
\[
y(x)=\log _2\left(\frac{3x+2}{x^2-5}\right){}^{1/4}=\frac{1}{4}\log _2(3x+2)-\frac{1}{4}\log _2\left(x^2-5\right)
\]
and then using derivative rules,  
\[
\frac{dy}{dx}=\frac{1}{4(3x+2)\ln (2)}\frac{d}{dx}(3x+2)-\frac{1}{4\left(x^2-5\right)\ln (2)}\frac{d}{dx}\left(x^2-5\right)\]
\[
\qquad =\frac{3}{4(3x+2)\ln (2)}-\frac{2x}{4\left(x^2-5\right)\ln (2)} 
=\frac{-3 x^2-4 x-15}{4 (3 x+2) \left(x^2-5\right) \ln (2)}
\square
\]
::: 


::: {#exm- }  
Find the derivative of the function given 
\[
s(t)=\log _5\left(\frac{t^2+3}{\sqrt{1-t}}\right).
\]
::: 

::: {.solution } Here we simplify first to have,  
\[
y(x)=\log _5\left(\frac{t^2+3}{\sqrt{1-t}}\right)=\log _5\left(t^2+3\right)-\frac{1}{2}\log _5(1-t)\
\]
and then using derivative rules,  
\[
\frac{dy}{dx}=\frac{2t}{\left(t^2+3\right)\ln (5)}-\frac{(-1)}{2\ln (5)(1-t)}=\frac{3 t^2-4 t-3}{2 (t-1) \left(t^2+3\right) \log (5)}
\square
\]
::: 

## Derivatives of Inverse Trigonometric Functions


::: {#thm- } 
The \index{inverse trigonometric functions} \index{arcsine}, \index{arccosine}, \index{arctangent}, \index{arccotangent}, \index{arccosecant}, and \index{arcsecant} **inverse trigonometric functions} \index{arcsine}, \index{arccosine}, \index{arctangent}, \index{arccotangent}, \index{arccosecant}, and \index{arcsecant**  are all differentiable functions on their domain and their derivative functions are:
\begin{align*}
& \frac{d}{d x}\sin ^{-1} x=\frac{1}{\sqrt{1-x^2}} & &
\frac{d}{d x}\cos ^{-1} x=\, -\frac{1}{\sqrt{1-x^2}} \\
& \frac{d}{d x}\tan ^{-1}x=\frac{1}{1+x^2} & &
\frac{d}{d x}\cot  ^{-1}x=\, -\frac{1}{1+x^2} \\
& \frac{d}{d x}\sec ^{-1}x=\frac{1}{|x|}\frac{1}{\sqrt{x^2-1}} & &
\frac{d}{d x}\csc ^{-1}x=\, -\frac{1}{|x|}\frac{1}{\sqrt{x^2-1}}
\end{align*}
::: 


::: {#exm- } 
Find the derivative of the function  $y=\sin ^{-1}x\text{  }\cos ^{-1}x.$
::: 

::: {.solution }
Using the product rule and the derivative formulas for arcsine and arccosine we determine:  
\[
y'=\left(\frac{1}{\sqrt{1-x^2}}\right)\left(\cos ^{-1}x\right)-\left(\frac{1}{\sqrt{1-x^2}}\right)\left(\sin  ^{-1}x\right)=\frac{\cos ^{-1}x-\sin^{-1}x}{\sqrt{1-x^2}}
\square
\]
::: 

::: {#exm- } 
Find the derivative of the function $y=\tan ^{-1}x\text{  }\cot ^{-1}x$
::: 

::: {.solution }
Using the product rule and the derivative formulas for arctangent and arccotangent we determine:  
\[
y'=\left(\frac{1}{1+x^2}\right)\cot ^{-1}x-\left(\frac{1}{1+x^2}\right)\tan ^{-1}x=\frac{\cot ^{-1}x-\tan ^{-1}x}{1+x^2}
\square
\]
::: 

::: {#exm- } 
Find the derivative of the function $y=\tan ^{-1}x-x \sec ^{-1}x$
::: 

::: {.solution }
Using the product rule and the derivative formulas for arctangent and arcsecant we determine: 
\[
y'=\left(\frac{1}{1+x^2}\right)-\sec ^{-1}x-x\left(\frac{1}{|x|}\frac{1}{\sqrt{x^2-1}}\right)
\square
\]
::: 

Recall, the \index{cofunction theorem} from trigonometry: if $\alpha =\cos  ^{-1}x$ and $\beta =\sin ^{-1} **cofunction theorem} from trigonometry: if $\alpha =\cos  ^{-1}x$ and $\beta =\sin ^{-1** x$ then $\cos  \alpha =\sin  \beta $ if and only if $\alpha +\beta =\pi /2.$


::: {#exm- } 
Find the derivative of the function $\ds y=\frac{\sin ^{-1}x}{\cos ^{-1}x}$.
::: 

::: {.solution } 
Using the quotient rule, the derivative formulas for arcsine and arccosine and some trigonometric identities, 
\begin{align*}
y'&=\frac{\left(\cos ^{-1}x\right)\left(\frac{1}{\sqrt{1-x^2}}\right)-\left(\sin ^{-1}x\right)\left(\frac{-1}{\sqrt{1-x^2}}\right)}{\left(\cos^{-1}x\right)^2} \\
& \qquad =\frac{\cos ^{-1}x+\sin ^{-1}x}{\left(\cos ^{-1}x\right)^2\sqrt{1-x^2}} 
=\frac{\pi }{2 \sqrt{1-x^2} \left(\cos ^{-1}x\right)^2}
\square
\end{align*}
::: 



## Exercises

::: {#exr- } 
Let $  f(x)=\frac{2x-3}{7-5x}.$ Sketch the graph of $f$ and state whether or not the graph of $f$ passes the \emph{horizontal line test}. If so, find a rule for $f^{-1}$ and then use it to find $\left(f^{-1}\right) '(0)$. Verify the formula $\left(f^{-1}\right)'(0)=\frac{1}{f '\left(f^{-1}(0)\right)}.$
::: 

::: {#exr- } 
Let $f(x)=\frac{5 x}{1-2x}.$ Without finding a rule for $f^{-1}(x)$ determine
 $\left(f^{-1}\right) '(1).$
::: 

::: {#exr- } 
Find $\frac{dy}{dx}$ given $  y=\frac{e^{2x}}{\left(x^2-3\right)^2\ln \sqrt{x}}.$
::: 

::: {#exr- } 
Find $\frac{dy}{dx}$ given $  y=x^{\sin  x}.$
::: 

::: {#exr- } 
Determine whether the following functions are one-to-one. 
 
- $f(x)=x^2+4$
- $f(x)=2x^3-4$ 
- $f(x)=-54+54 x-15 x^2+2 x^3$ \
- $  f(x)=\frac{2x-3}{x-7}$
 
::: 

::: {#exr- } 
Determine whether or not the given functions are inverses of each other or not.  
\ 
- $f(x)=x^3-4$ and  $g(x)=\sqrt[3]{x+4}$
- $f(x)=x^2+5, x\leq 0$  and  $g(x)=-\sqrt{x-5}, x\geq 5$
 
::: 

::: {#exr- } 
Find the inverse of the given function, it if exists.
 
- $f(x)=\frac{4x}{x-2}$
- $f(x)=\left(x^3+1\right)^5$
- $f(x)=x^2-6x, x\geq 3$
- $f(x)=\frac{x}{x^2-2}$
 
::: 

::: {#exr- } 
Solve the following equations for real $x$ and give the number of solutions you find for each one. Also clearly state any extraneous solutions that you find for each one.  
 
- $\log _2x=\log _45+3 \log _23$
- $\left(\sqrt[3]{5}\right)^{x+2}=5^{x^2}$ 
- $  \log _5|x+3|+\log _5|x-3|=1$ 
- $  \frac{1}{e^{x+3}+6e^{-x-3}}=\frac{1}{5}$
 
::: 

::: {#exr- } 
Given $f(x)=5-4x$ and $a=1/2$ find $f^{-1}(x)$ and graph $f$ and $f^{-1}$ together. Then evaluate $  \frac{ df}{dx}$ at $x=a$ and $  \frac{ df^{-1}}{dx}$ at $x=f(a)$ to show that at these points $  \frac{ d f^{-1}}{dx}=\frac{1}{\left(\frac{ df}{dx}\right)}.$
::: 

::: {#exr- } 
Show that $h(x)=\left.x^3\right/4$ and $k(x)=(4x)^{1/3}$ are inverses of one another. Graph $h$ an $k$ over an $x$-interval large enough to show the graphs intersecting at $(2,2)$ and $(-2,-2).$ Find the slopes of the tangents to the graphs at $h$ and $k$ at $(2,2)$ and $(-2,-2).$ What lines are tangent to the graphs at $h$ and $k$ at $(2,2)$ and $(-2,-2).$
::: 

::: {#exr- } 
Suppose that the differentiable function $y=f(x)$ has an inverse and that the graph of $f$ passes through the point $(2,4)$ and has a slope of $1/3$ there. Find the value of $  \frac{ df^{-1}}{dx}$ at $x=4.$
::: 


 

