---
pagetitle: "Limits Involving Infinity - Exploring Calculus"
---
# "Limits Involving Infinity"


## Infinite Limits

Infinite limits are used to described unbounded behavior of a function near a given real number which is not necessarily in the domain of the function. 
They are particularly useful for showing the intentions of the graph of a function by drawing dashed lines representing unbounded growth which are called vertical asymptotes.  

::: {#def- } 
Let $f$  be a function defined on both sides of $c,$  except possible at $c$  it self. 
Then $\lim _{x\to c}f(x)=+\infty $  means that the values of $f(x)$  can be made arbitrarily large by taking $x$  sufficiently close to $c$  ($x\neq c$ ).
::: 

::: {#def- } 
Let $f$  be a function defined on both sides of $c,$  except possible at $c$  itself. 
Then $\lim _{x\to c}f(x)=-\infty $  means that the values of $f(x)$  can be made arbitrarily large negative by taking $x$  sufficiently close to $c$  ($x\neq c$ ). 
::: 


::: {#exm- } 
Determine $\ds \lim _{x\to 0}\frac{1}{x}.$
::: 

::: {.solution }   
Since $f(x)=\frac{1}{x}$  decreases without bound as $x\to 0^-$ , we notice $\lim_{x\to 0^-}f(x)=-\infty$. 
Also since $f$  increases without bound as $x\to 0^+,$  we notice $\lim_{x\to 0^+}f(x)=+\infty$. 
Thus $\lim _{x\to0}f(x)$  does not exist. 
::: 

Compare the previous example with the following.


::: {#exm- }  
Determine $\ds \lim_{x\to2} \frac{2x^3+x^2-16x+12}{x^2-4}$.
::: 

::: {.solution }   
By factoring, 
\begin{align*}
& \lim _{x\to 2}\frac{2x^3+x^2-16x+12}{x^2-4} 
=\lim _{x\to 2}\frac{(x-2)\left(2x^2+5x-6\right)}{(x-2)(x+2)} \\
& \qquad =\lim _{x\to 2}\frac{\left(2x^2+5x-6\right)}{(x+2)}
=\frac{\left(2(2)^2+5(2)-6\right)}{((2)+2)} =3.
\square
\end{align*}
::: 


::: {#thm- }  
Let $A$  be a positive real number. 
 
- If $n$  is a positive even integer, then $\lim _{x\to c}\frac{A}{(x-c)^n}=+\infty.$ 
- If $n$  is a positive odd integer, then 
\[
\lim _{x\to c^+}\frac{A}{(x-c)^n}=+\infty 
\qquad \text{and} \qquad 
\lim _{x\to c^-}\frac{A}{(x-c)^n}=-\infty.
\]
 
::: 

::: {#exm- } 
Evaluate $\ds \lim _{x\to 2^+}\frac{-3}{\sqrt[3]{x-2}}$.
::: 

::: {.solution } 
Notice that $\ds \frac{1}{\sqrt[3]{x-2}}$  increases without bound as $x\to 2^+$  and therefore, $\ds \lim _{x\to 2^+}\frac{-3}{\sqrt[3]{x-2}}=-\infty.$ 
::: 

::: {#exm- } 
Evaluate $\ds \lim _{x\to 0}\left(\frac{1}{x}-\frac{1}{x^2}\right).$  
::: 

::: {.solution }   
Note that 
\[
f(x)=\frac{1}{x}-\frac{1}{x^2}=\frac{-1+x}{x^2}
\]  
and that $\frac{-1+x}{x^2}$ decreases without bound as $x\to 0^+$ and therefore, 
\[
\lim _{x\to 0^+}\frac{-1+x}{x^2}=-\infty.
\]
This is true because when $x>0$  is close to $0$  we know that $-1+x$  is negative. 
Similarly, $\lim _{x\to 0^-}\frac{-1+x}{x^2}=-\infty $  because when $x<0$  and close to $0$  we know that $-1+x$  is negative. 
Therefore it follows
\[
\lim _{x\to 0}\left(\frac{1}{x}-\frac{1}{x^2}\right)=-\infty
\] 
See Figure \eqref{fig:graph1}.
::: 

\begin{figure}[h]
\begin{center}
{\includegraphics[width=150pt]{_includes/p30.pdf}}
\caption{$f(x)=\frac{1}{x}-\frac{1}{x^2}$ }
\label{fig:graph1}
\end{center}
\end{figure}


## Vertical Asymptotes


::: {#def- } 
The line $x=c$  is called a \index{vertical asymptote} **vertical asymptote**  of the curve $y=f(x)$  if at least one of the following statements is true:
 {3}
& \lim _{x\to c}f(x)=+\infty &\qquad &  \lim _{x\to c^-}f(x)=+\infty &\qquad &  \lim _{x\to c^+}f(x)=+\infty  \\[10pt]
& \lim _{x\to c}f(x)=-\infty &\qquad & \lim _{x\to c^-}f(x)=-\infty &\qquad & \lim _{x\to c^+}f(x)=-\infty 
 
::: 

The following example demonstrates that not all rational functions have vertical asymptotes. 


::: {#exm- } 
Determine the vertical asymptotes of the function 
\[
g(x)=\frac{x^3}{x^2+3x+10}.
\]
::: 

::: {.solution }   
The function $g$  is continuous on its domain which is $\mathbb{R}$  and therefore there are no vertical asymptotes for this function. 
::: 


::: {#exm- } 
Determine the vertical asymptotes of the function 
\[
f(x)=\frac{x^3}{x^2+3x-10}.
\]
::: 

::: {.solution }  
Since 
\[
f(x)=\frac{x^3}{x^2+3x-10}=\frac{x^3}{(x-2)(x+5)}
\]
and therefore the vertical asymptotes are $x=2$  and $x=-5$  because
\[
\lim _{x\to 2^+}\frac{x^3}{(x-2)(x+5)}=+\infty 
\qquad \text{and} \qquad 
\lim _{x\to 5^+}\frac{x^3}{(x-2)(x+5)}=+\infty.
\square
\]
::: 

The following example demonstrates that there can be an unlimited number of vertical asymptotes for a function. 

::: {#exm- } 
Determine the vertical asymptotes of the function 
\[
h(x)=\tan  x-\cot  x.
\]
::: 

::: {.solution }   
We can rewrite this function as 
\[
h(x)=\tan  x-\cot  x=\frac{\sin  x}{\cos  x}-\frac{\cos  x}{\sin  x}=\frac{\sin ^2x-\cos ^2x}{\sin  x \cos  x}=\frac{\cos  2x}{\sin  x \cos x}.
\] 
Therefore the zeros of the sine and cosine functions yield the vertical asymptotes of $x=\pm \frac{\pi }{2}+k$  for all integers $k,$  since $\cos 2x$  is not zero for these values of $x$  and because, for any $c=\pm \frac{\pi }{2}+k$ , $\lim_{x\to c}h(x)$  is either $\pm \infty$. 
See Figure \eqref{fig:graph1}.
::: 

\begin{figure}[h]
\begin{center}
{\includegraphics[width=150pt]{_includes/p29.pdf}}
\caption{$h(x)=\tan x-\cot x$ }
\label{fig:graph2}
\end{center}
\end{figure}



## Limits at Infinity

::: {#def- } 
Let $f$  be a function defined on some interval $(a,+\infty ).$  
Then \[\lim _{x\to \infty }f(x)=L\] means that the values of $f(x)$  can be made arbitrarily close to $L$  by taking $x$  sufficiently large; or more precisely, for every $\epsilon>0$  there exists an $N$  such that if $x>N$  then $|f(x)-L|<\epsilon$. 
::: 

::: {#def- } 
Let $f$  be a function defined on some interval $(-\infty ,a).$ 
Then \[\lim _{x\to -\infty }f(x)=L\] means that the values of $f(x)$  can be made arbitrarily close to $L$  by taking $x$  sufficiently large negative; or more precisely, for every$\epsilon >0$  there exists an $N$  such that if $x<N$  then $|f(x)-L|<\epsilon.$  
::: 

The following limit rules are similar to the limit rules used for when $x\to c$  but instead use $x\to +\infty ;$  and they are also valid for when $x\to +\infty $  is replaced by $x\to -\infty.$ 

::: {#thm- } 
If $\lim _{x\to \infty }f(x)$  and $\lim _{x\to \infty }g(x)$  exist, then 
 
- $\lim _{x\to \infty } k=k$  for any constant $k$ 
- $\lim _{x\to \infty }k f(x)=k \lim _{x\to \infty }f(x)$ 
- $\lim _{x\to \infty }[f(x)+g(x)]=\lim _{x\to \infty }f(x)+\lim _{x\to \infty }g(x)$ 
- $\lim _{x\to \infty }[f(x)-g(x)]=\lim _{x\to \infty }f(x)-\lim _{x\to \infty }g(x)$ 
- $\lim _{x\to \infty }[f(x)g(x)]=\left( \lim _{x\to \infty }f(x) \right)\left( \lim _{x\to \infty }g(x) \right)$ 
- $\lim _{x\to \infty }[f(x)/g(x)]=\left( \lim _{x\to \infty }f(x) \right)/\left( \lim _{x\to \infty }g(x) \right)$ 
- $\lim _{x\to \infty }[f(x)]^n=\left( \lim _{x\to \infty }f(x) \right){}^n$  where $n$  is a rational number and whenever the limits exist. 
 
::: 

::: {#thm- } 
Let $A$  be a real number.
 
- If $r>0$  is a rational number, then 
\[
\lim _{x\to \infty }\frac{A}{x^r}=0.
\]
- If $r>0$  is a rational number with $x^r$  defined for all $x,$  then 
\[
\lim _{x\to -\infty }\frac{A}{x^r}=0.
\]
 
::: 


::: {#exm- } 
Evaluate $\ds\lim _{x\to \infty }\frac{3x^2-x-2}{5x^2+4x+1}.$ 
::: 

::: {.solution }   
To evaluate this limit we divide both the numerator and the denominator by the highest power of $x$  that occurs. 
So we have
\[
\lim _{x\to \infty }\frac{3x^2-x-2}{5x^2+4x+1}
=\lim _{x\to \infty }\frac{\frac{3x^2}{x^2}-\frac{x}{x^2}-\frac{2}{x^2}}{\frac{5x^2}{x^2}+\frac{4x}{x^2}+\frac{1}{x^2}}
=\lim _{x\to \infty }\frac{3-\frac{1}{x}-\frac{2}{x^2}}{5+\frac{4}{x}+\frac{1}{x^2}}
% =\frac{3-0-0}{5+0+0}
=\frac{3}{5}.
\]
::: 


::: {#exm- } 
Evaluate $\ds \lim _{x\to \infty }\left(x-\sqrt{x^2+1}\right).$ 
::: 

::: {.solution }  
We use the conjugate radical as follows
\begin{align*}
& \lim _{x\to \infty }\left(x-\sqrt{x^2+1}\right)
=\lim _{x\to \infty }\frac{\left(x-\sqrt{x^2+1}\right)\left(x+\sqrt{x^2+1}\right)}{\left(x+\sqrt{x^2+1}\right)} \\
& \qquad  =\lim _{x\to \infty }\frac{x^2-\left(x^2+1\right)}{\left(x+\sqrt{x^2+1}\right)}
=\lim _{x\to \infty }\frac{-1}{x+\sqrt{x^2+1}} \\
& \qquad  =\lim _{x\to \infty }\frac{\frac{-1}{x}}{\frac{x}{x}+\sqrt{\frac{x^2+1}{x^2}}}
=\frac{0}{1+\sqrt{1+0}}=0.
\square
\end{align*}
::: 




## Horizontal Asymptotes

In mathematics, the symbol $\infty $  is not a number, rather it is used to describe the process of unrestricted growth or the result of such a growth.

::: {#def- } 
The line $y=L$  is called a \index{horizontal asymptote} of the curve $y=f(x)$  if either $\lim _{x\to \infty }f(x)=L$   or  $\lim _{x\to -\infty } **horizontal asymptote} of the curve $y=f(x)$  if either $\lim _{x\to \infty }f(x)=L$   or  $\lim _{x\to -\infty ** f(x)=L.$ 
::: 

::: {#thm- }  If $f$  is a rational functions of the form:  
\[
f(x)=\frac{a_0+a_1x+a_2x^2+\cdots +a_nx^n}{b_0+b_1x+b_2x^2+\cdots +b_mx^m}
\]
where $n$  is the degree of the polynomial in the numerator and $m$  is the degree of the polynomial in the denominator, then the horizontal asymptote of the curve $y=f(x)$  is determined by the following. 
 
- If $n=m,$  then $y=\frac{a_n}{b_m}$  is the horizontal asymptote. 
- If $n<m,$  then $y=0$  is the horizontal asymptote. 
- If $n>m,$  then there is no horizontal asymptote, but rather a slant (oblique) asymptote and can be found be using long division.
 
::: 


::: {#exm- } 
Find the horizontal asymptote of the graph of the function 
\[
f(x)=\frac{(1-x)(2+x)}{(1+2x)(2-3x)}.
\]
::: 

::: {.solution }   
The degree of the numerator $(1-x)(2+x)=-x^2-x+2$  is 2 and the degree of the denominator $(1+2x)(2-3x)=-6 x^2+x+2$  is 2 we
divide both numerator and denominator by $x^2$  and using the properties of limits, we have 
\[
%\lim_{x\to \infty} f(x)=
\lim_{x\to \pm\infty} \frac{-x^2-x+2}{-6 x^2+x+2}=
%\lim_{x\to \pm\infty} \frac{\frac{-x^2-x+2}{x^2}}{\frac{-6 x^2+x+2}{x^2}}=
\lim_{x\to \pm\infty} \frac{\frac{-x^2}{x^2}-\frac{x}{x^2}+\frac{2}{x^2}}{\frac{-6 x^2}{x^2}+\frac{x}{x^2}+\frac{2}{x^2}}=
\frac{-1-0+0}{-6+0+0}=6
\]
Therefore the only horizontal asymptote of the graph of $f(x)$  is $y=6.$ 
::: 


::: {#exm- } 
Find the horizontal asymptote of the graph of the function 
\[
f(x)=\frac{\sqrt{2x^2+1}}{3x-5}.
\]
::: 

::: {.solution }   
Dividing both numerator and denominator by $x$  and using the properties of limits, we have 
\begin{align*}
\lim _{x\to \infty }\frac{\sqrt{2x^2+1}}{3x-5}
=\lim _{x\to \infty }\frac{\sqrt{2+\frac{1}{x^2}}}{3-\frac{5}{x}} 
=\frac{\sqrt{\lim _{x\to \infty }\left(2+\frac{1}{x^2}\right)}}{\lim _{x\to \infty }\left(3-\frac{5}{x}\right)}
=\frac{\sqrt{2+0}}{3-5(0)}=\frac{\sqrt{2}}{3}
\end{align*}
Therefore the line $y=\left.\sqrt{2}\right/3$  is a horizontal asymptote. 
It is also important to realize that 
\begin{align*}
 \lim _{x\to -\infty }\frac{\sqrt{2x^2+1}}{3x-5}
& =\lim _{x\to -\infty }\frac{\frac{1}{x}\sqrt{2x^2+1}}{3-\frac{5}{x}} \\
& =\lim _{x\to -\infty }\frac{\left(\frac{-1}{\sqrt{x^2}}\right)\sqrt{2x^2+1}}{3-\frac{5}{x}} 
=\lim _{x\to -\infty }\frac{-\sqrt{2+\frac{1}{x^2}}}{3-\frac{5}{x}} 
=-\frac{\sqrt{2}}{3}
\end{align*}
Therefore, the line $y=\left.-\sqrt{2}\right/3$  is another horizontal asymptote. 
::: 


::: {#exm- }  
Find all horizontal asymptotes of the graph of the function 
\[
f(x)=\frac{x}{\sqrt[4]{x^4+1}}.
\]
::: 

::: {.solution }   
Dividing both numerator and denominator by $x$  and using the properties of limits, we have 
\begin{align*}
\lim _{x\to \infty }\frac{x}{\sqrt[4]{x^4+1}}
& =\lim _{x\to \infty }\frac{\frac{x}{x}}{\frac{1}{x}\sqrt[4]{x^4+1}} 
=\lim _{x\to \infty }\frac{1}{\sqrt[4]{\frac{x^4+1}{x^4}}} \\
& =\lim _{x\to \infty }\frac{1}{\sqrt[4]{1+\frac{1}{x^4}}}
=\frac{1}{\sqrt[4]{\lim _{x\to \infty }\left(1+\frac{1}{x^4}\right)}}
=\frac{1}{\sqrt[4]{1+0}}=1.
\end{align*}
Therefore, the line $y=1$  is a horizontal asymptote. 
In computing the limit $x\to -\infty $ we must remember that for $x<0,$  we have $\sqrt[4]{x^4}=-x,$  so when we divide the numerator by $x,$  when $x<0$  we have, 
\begin{align*}
 \lim _{x\to -\infty }\frac{x}{\sqrt[4]{x^4+1}}
& =\lim _{x\to -\infty }\frac{\frac{x}{x}}{\frac{1}{x}\sqrt[4]{x^4+1}} \\
& =\lim _{x\to \infty }\frac{1}{\frac{1}{\sqrt[4]{x^4}}\sqrt[4]{\frac{x^4+1}{x^4}}}
=\lim _{x\to \infty }\frac{1}{-\text{  }\sqrt[4]{1+\frac{1}{x^4}}}
=-1.
\end{align*}
Therefore, the horizontal asymptotes are $y=\pm 1.$  
::: 


