---
pagetitle: "Tangent Planes and Normal Lines - Exploring Calculus"
---
# Tangent Planes and Normal Lines


## Tangent Planes

Suppose $S$ is a surface with the equation $z=f(x,y)$ where $f$ has continuous first partial derivatives $f_x$ and $f_y$. 
Let $P(a,b,c)$ be a point on $S$ and let $C_1$be the curve of intersection of $S$ with the plane $x=a$ and $C_2$ the intersection of $S$ with the plane $y=b$. 
The tangent lines $T_1$ and $T_2$ to $C_1$ and $C_2$, respectively determine a unique plane and this plane actually contains the tangent to every smooth curve $C$ that passes through $P.$ 
We call this plane the \index{tangent plane} **tangent plane**  to $S$ at $P$.


::: {#thm- } [Equation of Tangent Plane]
If $z=f(x,y)$ is differentiable at $(a,b)$ then an equation of the tangent plane to the graph of $f$ at $(a,b)$ is 
\[
z-f(a,b)=f_x(a,b)(x-a)+f_y(a,b)(y-b).
\]
::: 

::: {.proof }
The proof is left for the reader.
::: 

\begin{figure}[htb]
\centering
\includegraphics{_includes/tpex5.pdf}
\caption{The surface $z=2x^2+y^2$ and its tangent plane at $(1,1,3)$.}
\label{fig:tanplane-1}
\end{figure} 


::: {#exm- } 
Find an equation of the tangent plane to the surface 
$$
z=2x^2+y^2
$$ 
at the point $(1,1,3)$.
::: 

::: {.solution }
Let $f(x,y)=2x^2+y^2.$ 
Then 
$$
f_x(x,y)=4x, \quad 
f_x(1,1)=4, \quad 
f_y(x,y)=2y, \quad
f_y(1,1)=2. 
$$
Then an equation of the tangent
plane is $z-3=4(x-1)+2(y-1)$ or 
\begin{equation}
z=4x+2y-3.
\tag*{}
\end{equation}
::: 

\begin{figure}[htb]
\centering
\includegraphics{_includes/tpex6.pdf}
\caption{The surface $z=$$
z=4-x^2-y^2$ and its tangent plane at $(1,1,2)$.}
\label{fig:tanplane-2}
\end{figure} 

::: {#exm- } 
Find an equation of the tangent plane to the surface 
$$
z=4-x^2-y^2
$$ 
at the point $(1,1,2)$. 
::: 

::: {.solution }
Let $f(x,y)=4-x^2-y^2.$ 
Then 
$$
f_x(x,y)=-2x, \quad 
f_x(1,1)=-2, \quad 
f_y(x,y)=-2y, \quad
f_y(1,1)=-2. 
$$
Then an equation of the tangent
plane is $z-2=-2(x-1)-2(y-1)$ or 
\begin{equation}
z=-2x-2y+6
\tag*{}
\end{equation}
::: 

\begin{figure}[htb]
\centering
\includegraphics{_includes/tpex7.pdf}
\caption{The surface $z=$$
z=\sin x+\sin y$ and its tangent plane at $\left(\frac{\pi}{2},\frac{\pi}{3},1+\frac{\sqrt{3}}{2}\right)$.}
\label{fig:tanplane-3}
\end{figure} 

::: {#exm- } 
Find an equation of the tangent plane to the surface 
$$
z=\sin x+\sin y
$$ 
at the point $\left(\frac{\pi}{2},\frac{\pi}{3},1+\frac{\sqrt{3}}{2}\right)$. 
::: 

::: {.solution }
Let $f(x,y)=\sin x+\sin y$. 
Then 
$$
f_x(x,y)=\cos x, \quad 
f_x\left(\frac{\pi}{2},\frac{\pi}{3}\right)=0, \quad 
f_y(x,y)=\cos y, \quad
f_y\left(\frac{\pi}{2},\frac{\pi}{3}\right)=\frac{1}{2}.
$$
Then an equation of the tangent
plane is 
$$
z-\left(1+\frac{\sqrt{3}}{2}\right)=0\left(x-\frac{\pi}{2}\right)+\frac{1}{2}\left(y-\frac{\pi}{3}\right)
$$ 
or 
\begin{equation}
z=\frac{1}{2}y-\frac{\pi}{6}+1+\frac{\sqrt{3}}{2}
\tag*{}
\end{equation}
::: 


::: {#thm- } [Tangent Plane To A Surface]
Suppose $S$ is a surface with the equation $F(x,y,z)=C$ and let $P(a,b,c)$ be a point on $S$ where $F$ is differentiable with $\nabla F_P\neq 0.$ Then an equation of the tangent plane to $S$ at $P$ is
\[
F_x(a,b,c)(x-a)+F_y(a,b,c)(y-b)+F_z(a,b,c)(z-c)=0
\]  
and the normal line to $S$ at $P$ has parametric equations 
\[
x=a+F_x(a,b,c) t, \qquad 
y=b+F_y(a,b,c) t, \qquad 
z=c+F_z(a,b,c) t.\]
::: 
 
::: {.proof }
Any plane that passes through $P(a,b,c)$ has an equation of the form 
$$
A(x-a)+B(y-b)+C(z-c)=0.
$$ 
By dividing this equation by $C$
and letting $a_1=-A/C$ and $b_1=-B/C$, we can write it in the form 
$$
z-c=a_1(x-a)+b_1(y-b).
$$ 
If this equation represents the tangent plane at
$P$, then its intersection with the plane $y=b$ must be the tangent line with slope $f_x(a,b)$. 
Therefore, $a_1=f_x(a,b).$ 
Similarly, putting
$x=a$, we get $z-c=b_2(y-b),$ which must represent the tangent line with slope $f_y(a,b)$ and so $b_2=f_y(a,b).$ 
Thus, the equation of
the tangent plane is $z-c=f_x(a,b)(x-a)+f_y(a,b)(y-b).$ 
::: 


::: {#exm- } 
Find an equation of the tangent plane to the surface 
\[
\frac{x^2}{a^2}+\frac{y^2}{b^2}+\frac{z^2}{c^2}=1
\]
at the point $(x_0,y_0,z_0)$.
::: 

::: {.solution }
Since 
$F_x=2x/a^2,$ 
$F_y=2y/b^2,$ and 
$F_z=2z/c^2,$ 
the tangent plane at $P_0\left(x_0,y_0,z_0\right)$ has equation  
\[
\frac{2x_0}{a^2}\left(x-x_0\right)+\frac{2y_0}{b^2}\left(y-y_0\right)+\frac{2z_0}{c^2}\left(z-z_0\right)=0\]
\[
\frac{x_0 x}{a^2}-\frac{x_0{}^2}{a^2}+\frac{y_0y}{b^2}-\frac{y_0^2}{b^2}+\frac{z_0z}{c^2}-\frac{z_0{}^2}{c^2}=0\]
\[
\frac{x_0 x}{a^2}+\frac{y_0y}{b^2}+\frac{z_0z}{c^2}=1.
\]
::: 

::: {#exm- } 
Find an equation of the tangent plane to the surface 
 \[
\frac{x^2}{a^2}+\frac{y^2}{b^2}-\frac{z^2}{c^2}=1
\] 
at the point $(x_0,y_0,z_0)$.
::: 

::: {.solution }
Since 
$F_x=2x/a^2,$ 
$F_y=2y/b^2,$ and 
$F_z=-2z/c^2,$ 
the tangent plane at $P_0\left(x_0,y_0,z_0\right)$ has equation  
\[
\frac{2x_0}{a^2}\left(x-x_0\right)+\frac{2y_0}{b^2}\left(y-y_0\right)-\frac{2z_0}{c^2}\left(z-z_0\right)=0\]
\[
\frac{x_0 x}{a^2}-\frac{x_0^2}{a^2}+\frac{y_0y}{b^2}-\frac{y_0^2}{b^2}+\frac{z_0z}{c^2}+\frac{z_0^2}{c^2}=0\]
\[
\frac{x_0 x}{a^2}+\frac{y_0y}{b^2}-\frac{z_0z}{c^2}=1.
\]
::: 

::: {#exm- } 
Find an equation of the tangent plane to the surface 
\[
\frac{z}{c}=\frac{x^2}{a^2}+\frac{y^2}{b^2}
\]
at the point $(x_0,y_0,z_0)$.
::: 

::: {.solution }
Since 
$F_x=2x/a^2,$ 
$F_y=2y/b^2,$ and 
$F_z=-1/c,$ 
the tangent plane at $P_0\left(x_0,y_0,z_0\right)$ has equation
\[
\frac{2x_0}{a^2}\left(x-x_0\right)+\frac{2y_0}{b^2}\left(y-y_0\right)-\frac{1}{c}\left(z-z_0\right)=0\]
\[
\frac{x_0 x}{a^2}-\frac{x_0^2}{a^2}+\frac{y_0y}{b^2}-\frac{y_0{}^2}{b^2}+\frac{z}{c}+\frac{z_0}{c}=0
\] 
\[
\frac{x_0 x}{a^2}+\frac{y_0y}{b^2}-\frac{z}{c}=\frac{z_0}{c}.
\]
::: 

## Normal Lines


::: {#exm- } 
Find the equations for the tangent plane and the normal line to the cone 
$$
z^2=x^2+y^2
$$ 
at the point where $x=3, y=4,$ and $z>0.$
::: 

::: {.solution }
If $P(a,b,c)$ is the point of tangency and $a=3, y=4,$ and $c>0,$ then $c=\sqrt{a^2+b^2}=5.$ 
If we consider $F(x,y,z)=x^2+y^2-z^2,$
then the cone can be regarded as the level surface $F(x,y,z)=0.$ 
The partial derivatives of $F$ are $F_x=2x$, $F_y=2y $, and $F_z=-2z$
so at $P(3,4,5)$ we find $F_x(3,4,5)=6$, $F_y(3,4,5)=8,$ and $F_z(3,4,5)=-10.$ Thus the tangent plane has an equation 
\[6(x-3)+8(y-4)-10(z-5)=0\]
or $3x+4y-5z=0$ and the normal line is given parametrically by the equations $x=3+6t ,$ $y=4+8t,$ and $z=5-10t.$ 
::: 


::: {#exm- } 
Find the equations of the tangent plane and the normal line at the point $(-2,1,-3)$ to the ellipsoid 
$$
\frac{x^2}{4}+y^2+\frac{z^2}{9}=3.
$$
::: 

::: {.solution }
The ellipsoid is a level surface of the function 
$$
F(x,y,z)=\frac{x^2}{4}+y^2+\frac{z^2}{9}.
$$ 
Therefore we have  
\[
F_x(x,y,z)=\frac{x}{2}, \quad 
F_y(x,y,z)=2y, \quad 
F_z(x,y,z)=\frac{2z}{9}
\]
Thus, 
$$
F_x(-2,1,3)=-1, \quad 
F_y(-2,1,3)=2, \quad F_z(-2,1,3)=-2/3.
$$  
Then the tangent plane at $(-2,1,-3)$ is 
$$
-1(x+2)+2(y-1)-(2/3)(z+3)=0
$$ 
which simplifies to 
$$
3x-6y+2z+18=0
$$ 
and parametric equations for the normal line are 
$$
x=-2- t, \quad 
y=1+2t, \quad 
z=-3-(2/3)t.
$$
::: 

## Exercises

::: {#exr- } 
Find the directional derivative of $f(x,y)=x^2y^2-x^2+2y$ at the point $(2,2)$ in the direction of the unit vector $\vec{u}=\frac{1}{2}\vec{i}-\frac{\sqrt{3}}{2}\vec{j}$.
::: 

::: {#exr- } 
Find the gradient of the function $f(x,y)=y \tan  x+\sin xy$.
::: 

::: {#exr- } 
Find the directional directive of $ f(x,y)=\frac{e^{-x}}y$ at $P(0,-1)$ in the direction of $\mathbf{v}=-\mathbf{i}+\mathbf{j}$.
::: 

::: {#exr- } 
Find the gradient of the function.
 
- $f(x,y)=x^2-2 x y$
- $f(x,y)=\ln \left(x^2+y^2\right)$
- $f(x,y)=\sin (x+2y)$ 
- $f(x,y,z)=\frac{x y-1}{z+x}$
- $f(x,y,z)= x y z^2$
- $g(x,y,z)=x e^{y+3z}$
    
::: 

::: {#exr- } 
Compute the directional derivative of the function $f(x,y)=\ln \left(x^2+3y\right)$ at the point $(1,1)$ in the direction of the vector $v=\vec{i}+\vec{j}.$
::: 

::: {#exr- } 
Compute the directional derivative of the function $f(x,y)=\sin  x y$ at the point $\left(\sqrt{\pi },\sqrt{\pi }\right)$ in the direction of the vector $v=3\pi  \vec{i}-\pi  \vec{j} .$
::: 

::: {#exr- } 
Find the directional derivative of the given function at the given point in the direction of the given vector.  
 
- $f(x,y)=x^2+x y$, $(1,-2),$ and $\vec{i}+\vec{j}$ 
- $f(x,y)=\frac{e^{-x}}{y},$ $(2,-1),$ and $-\vec{i}+\vec{j}$
    
::: 

::: {#exr- } 
Find the directional derivative of the given function at the given point in the direction of the given vector. 
 
- $f(x,y)=\ln \left(3x+y^2\right)$, $(0,1),$ and $\vec{i}-\vec{j}$  
- $f(x,y)=\sec \left(x y-y^3\right),$ $(2,0),$ and $-\vec{i}-3\vec{j}$
 
::: 

::: {#exr- } 
Find the direction from $P_0$ in which the given function $f$ increases most rapidly and compute the magnitude of the greatest rate of increase. 
 
- $f(x,y,z)=(x+y)^2+(y+z)^2+(x+z)^2$ at $P_0(2,-1,2)$  
- $f(x,y,z)=z \ln \left(\frac{y}{z}\right)$ at $P_0(1,e,-1)$
    
::: 


